Imp optmizer

src/Refine2.v
@@ -35,16 +35,6 @@ Next Obligation.
 refine (forall y, x y = 2).
 Defined.
 
-Definition swap_spec: Eff [State state] unit :=
-  st <- send Get;
-  send (Put (st & {X --> st Y; Y --> st X}));;
-  pure tt.
-
-Definition swap_impl: com :=
-  X ::= Y ;;;
-  Y ::= X.
-
-
 Fixpoint denote_aexp `{Member (State state) effs}
          (a:aexp): Eff effs nat :=
   match a with
@@ -96,7 +86,109 @@ Fixpoint denote_imp `{Member (State state) effs}
   | WHILE b DO c' END => pure tt (* <- bogus *)
   end.
 
-Eval simpl in (denote_imp swap_impl).
+Definition swap_spec1: Eff [State state] unit :=
+  st <- send Get;
+  send (Put (st & {W --> st Y; X --> st Y}));;
+  pure tt.
+
+Definition swap_spec2: Eff [State state] unit :=
+  st <- send Get;
+  send (Put (st & {W --> st Y}));;
+  st' <- send Get;
+  send (Put (st' & {X --> st' Y}));;
+  pure tt.
+
+Definition swap_impl: com :=
+  W ::= Y;;;
+  X ::= Y.
+
+Eval cbn in (denote_imp swap_impl).
+Eval cbn in swap_spec1.
+
+(* Write a function to transform 
+ * (fun x => 1 + (fun y => x + y))
+ * into ~~~>
+ * (fun x => 1 + x + x)
+*)
+
+Definition blah: (nat -> nat -> nat) -> nat -> nat :=
+  fun f x => f x x.
+
+Program Fixpoint merge_impures `(e: Eff (State state :: effs) v): Eff (State state :: effs) v :=
+  match e with
+  | Pure x => pure x
+  | Impure u k => let default := (fun x => merge_impures (k x)) in
+                 match decomp u with
+                 | inl st =>
+                   match st with
+                   | Get => Impure u (fun x =>
+                                       match k x with
+                                       | Pure x => pure x
+                                       | Impure u' k' =>
+                                         match decomp u' with
+                                         | inl st' =>
+                                           match st' with
+                                           | Get => merge_impures (k' _)
+                                           | Put y => merge_impures (k x)
+                                           end
+                                         | _ => merge_impures (k x)
+                                         end
+                                       end)
+                   | Put x => Impure u default
+                   end
+                 | _ => Impure u default
+                 end
+  end.
+
+Eval cbn in (merge_impures (denote_imp swap_impl)).
+Eval cbn in swap_spec1.
+Eval cbn in swap_spec2.
+
+Lemma swap_respects_spec2:
+  merge_impures (denote_imp swap_impl) = swap_spec2.
+Proof.
+  reflexivity.
+Qed.
+Require Import Coq.Logic.FunctionalExtensionality.
+
+Lemma swap_disrespects_spec2:
+  merge_impures (denote_imp swap_impl) <> swap_spec1.
+Proof.
+  intro.
+  inversion H.
+  apply inj_pair2 in H1.
+  eapply equal_f in H1.
+  inversion H1.
+  apply inj_pair2 in H2.
+Admitted.
+
+
+
+Definition merge_impures {effs f x a}: (forall x, f x -> (x -> Eff effs a)) -> 
+
+     = Impure (UThis Get)
+         (fun x : string -> nat =>
+          Impure (UThis Get)
+            (fun x0 : total_map nat =>
+             Impure (UThis (Put (x0 & {X --> x Y}))) (fun _ : () => Pure ())))
+
+Lemma normalize_nat : forall (a b: nat),
+  ((fun x => (fun y => x + x)) a b) = (fun x => x + x).
+Proof.
+  intros.
+  simpl.
+  reflexivity.
+Qed.
+
+Fixpoint normalize_r `(e: Eff (State v :: effs) unit) (b: bool) (c: v)
+  : Eff (State v :: effs) unit :=
+  match e with
+  | Pure x => pure x
+  | Impure u (fun x => k) => match decomp u with
+                         | inl l => _
+                         end
+  end.
+
 
 
 Definition refines {a effs} (e1 e2: Eff effs a) := 
